add Montgomery arithmetic

specs/experimental/Spec.RSA.Test.fst
@@ -27,6 +27,7 @@ let ctest modBits nLen n eLen e dLen d pLen p qLen q msgLen msg sLen salt rBlind
 	let verify_sgnt = rsa_verify modBits pkey sLen sgnt msgLen msg in
     check_sgnt && verify_sgnt
 
+val test1: unit -> bool
 let test1() =
 	let msg = List.Tot.map u8_from_UInt8 [
 	 	0x85uy; 0x13uy; 0x84uy; 0xcduy; 0xfeuy; 0x81uy; 0x9cuy; 0x22uy; 0xeduy; 0x6cuy; 0x4cuy; 0xcbuy; 0x30uy; 0xdauy; 0xebuy; 0x5cuy; 
@@ -89,6 +90,7 @@ let test1() =
 	let sgnt_expected : lbytes 128 = createL sgnt_expected in
     ctest 1024 128 n 3 e 128 d 64 p 64 q 51 msg 20 salt 45 rBlind sgnt_expected
 
+val test2: unit -> bool
 let test2() =
     let n = List.Tot.map u8_from_UInt8 [
         0x01uy; 0xd4uy; 0x0cuy; 0x1buy; 0xcfuy; 0x97uy; 0xa6uy; 0x8auy; 0xe7uy; 0xcduy; 0xbduy; 0x8auy; 0x7buy; 0xf3uy; 0xe3uy; 0x4fuy;
@@ -166,6 +168,7 @@ let test2() =
     let sgnt_expected : lbytes 129 = createL sgnt_expected in
     ctest 1025 129 n 3 e 128 d 65 p 65 q 234 msg 20 salt 38 rBlind sgnt_expected
 
+val test3: unit -> bool
 let test3() = 
     let n = List.Tot.map u8_from_UInt8 [
         0xe6uy; 0xbduy; 0x69uy; 0x2auy; 0xc9uy; 0x66uy; 0x45uy; 0x79uy; 0x04uy; 0x03uy; 0xfduy; 0xd0uy; 0xf5uy; 0xbeuy; 0xb8uy; 0xb9uy;
@@ -247,6 +250,7 @@ let test3() =
     let sgnt_expected : lbytes 192 = createL sgnt_expected in
     ctest 1536 192 n 3 e 192 d 96 p 96 q 107 msg 20 salt 48 rBlind sgnt_expected
 
+val test4: unit -> bool
 let test4() = 
     let n = List.Tot.map u8_from_UInt8 [
         0xa5uy; 0xdduy; 0x86uy; 0x7auy; 0xc4uy; 0xcbuy; 0x02uy; 0xf9uy; 0x0buy; 0x94uy; 0x57uy; 0xd4uy; 0x8cuy; 0x14uy; 0xa7uy; 0x70uy;
@@ -345,14 +349,5 @@ let test4() =
     let sgnt_expected : lbytes 256 = createL sgnt_expected in
     ctest 2048 256 n 3 e 256 d 128 p 128 q 128 msg 20 salt 35 rBlind sgnt_expected
 
-let test_exp() =
-    let n = 92086691 in
-    let e = 21954739 in
-    let d = 40692523 in
-    let m = 4567389 in
-    let s = mod_exp n m d in
-    let m1 = mod_exp n s e in
-    m = m1
-
-let test() =
-    test_exp() && test1() && test2() && test3() && test4()
+val test: unit -> bool
+let test() = test1() && test2() && test3() && test4()
